test/mllist.lean
@@ -1,0 +1,18 @@
+import tidy.mllist
+
+open mllist
+
+meta def f : nat → tactic nat
+| 0 := tactic.failed
+| (n+1) := tactic.trace n $> n
+
+run_cmd fix f 10 -- prints only 9
+
+run_cmd (fix f 10 >>= mllist.force >>= tactic.trace) -- prints 9,...,0 and [9, ..., 0]
+
+run_cmd (do L ← fix f 10, L ← L.map (λ n, n*n), mllist.force L >>= tactic.trace) -- prints 9,...,0 and [81, ..., 0]
+
+meta def g : nat → tactic nat
+| n := tactic.trace ("g " ++ (to_string n)) $> (n*n)
+
+run_cmd (do L ← fix f 10, L ← L.mmap g, mllist.force L >>= tactic.trace) -- prints 9,...,0 and [81, ..., 0]
